Termino clase 05

Clase05.BST.fst
@@ -101,9 +101,35 @@ let rec member (x: int) (t: bst) : bool =
     else if x > y then member x r
     else true
 
-let member_ok (x:int) (t:bst) : Lemma (member x t == in_tree x t) =
-  admit()
+let rec all_lt_not_in_tree (x:int) (t:bst) (y:int) : Lemma (requires x > y /\ all_lt y t) 
+                                                           (ensures ~ (in_tree x t)) =
+  match t with
+  | L -> ()
+  | N (l,_,r) -> all_lt_not_in_tree x l y;
+                 all_lt_not_in_tree x r y 
 
+let rec all_gt_not_in_tree (x:int) (t:bst) (y:int) : Lemma (requires x < y /\ all_gt y t)
+                                                           (ensures ~ (in_tree x t)) =
+  match t with
+  | L -> ()
+  | N (l,_,r) -> all_gt_not_in_tree x l y;
+                 all_gt_not_in_tree x r y 
+
+let rec member_ok (x:int) (t:bst) : Lemma (member x t == in_tree x t) =
+  match t with 
+  | L -> ()
+  | N (l, y, r) ->
+    if x = y then ()
+    else if x < y 
+         then (
+              all_gt_not_in_tree x r y;
+              member_ok x l;
+              ()
+         ) else (
+              all_lt_not_in_tree x l y;
+              member_ok x r;
+              ()
+              )
 let rec to_list (t: bst) : list int =
   match t with
   | L -> []
@@ -147,11 +173,21 @@ let rec insert_mem (x:int) (t:bst) : Lemma (member x (insert x t)) =
     then insert_mem x l
     else insert_mem x r
 
-let all_lt_trans (x y : int) (t : bst0) : Lemma (requires all_lt x t /\ y >= x) (ensures all_lt y t) =
-  admit()
+let rec all_lt_trans (x y : int) (t : bst0) : Lemma (requires all_lt x t /\ y >= x) (ensures all_lt y t) =
+  match t with
+  | L -> ()
+  | N (l, _, r) ->
+    all_lt_trans x y l;
+    all_lt_trans x y r;
+    ()
 
-let all_gt_trans (x y : int) (t : bst0) : Lemma (requires all_gt x t /\ y <= x) (ensures all_gt y t) =
-  admit()
+let rec all_gt_trans (x y : int) (t : bst0) : Lemma (requires all_gt x t /\ y <= x) (ensures all_gt y t) =
+  match t with
+  | L -> ()
+  | N (l, _, r) ->
+    all_gt_trans x y r;
+    all_gt_trans x y l;
+    ()
 
 // NB: cambiado para fortalecer la precondición, y no devolver una opción.
 let rec extract_min0 (t: bst0{N? t}) : int & bst0 =
@@ -162,19 +198,27 @@ let rec extract_min0 (t: bst0{N? t}) : int & bst0 =
     let t : bst0 = N (l', x, r) in
     (min, t)
 
-let extract_min_preserva_all_lt (y:int) (t : bst0{N? t})
+let rec extract_min_preserva_all_lt (y:int) (t : bst0{N? t})
   : Lemma (requires is_bst t /\ all_lt y t)
           (ensures all_lt y (snd (extract_min0 t)))
-= admit()
+= 
+  match t with
+  | N (L, x, r) -> ()
+  | N (l, x ,r) -> extract_min_preserva_all_lt y l
 
-let extract_min_es_bst (t:bst0{N? t})
+
+let rec extract_min_es_bst (t:bst0{N? t})
 : Lemma (requires is_bst t)
         (ensures is_bst (snd (extract_min0 t)))
-=
-  admit()
+= match t with
+  | N (L, x, r) -> ()
+  | N (l, x, r) -> extract_min_es_bst l;
+                   extract_min_preserva_all_lt x l
 
 let extract_min (t: bst{N? t}) : (int & bst) =
-  admit()
+  extract_min_es_bst t;
+  let (m, t') = extract_min0 t in
+  (m, t')
 
 let delete_root0 (t: bst0{N? t}) : bst0 =
   let N (l, _, r) = t in
